src/lang/Thread.v
@@ -26,21 +26,21 @@ Module Local.
     mk Commit.init
        Memory.bot.
 
-  Inductive is_terminal (th:t): Prop :=
+  Inductive is_terminal (lc:t): Prop :=
   | is_terminal_intro
-      (PROMISE: th.(promise) = Memory.bot)
+      (PROMISE: lc.(promise) = Memory.bot)
   .
 
-  Inductive wf (th:t) (mem:Memory.t): Prop :=
+  Inductive wf (lc:t) (mem:Memory.t): Prop :=
   | wf_intro
-      (COMMIT: Commit.wf th.(commit) mem)
-      (PROMISE: Memory.le th.(promise) mem)
+      (COMMIT: Commit.wf lc.(commit) mem)
+      (PROMISE: Memory.le lc.(promise) mem)
       (MEMORY: Memory.wf mem)
   .
 
-  Inductive disjoint (th1 th2:t): Prop :=
+  Inductive disjoint (lc1 lc2:t): Prop :=
   | disjoint_intro
-      (PROMISE: Memory.disjoint th1.(promise) th2.(promise))
+      (PROMISE: Memory.disjoint lc1.(promise) lc2.(promise))
   .
 
   Global Program Instance disjoint_Symmetric: Symmetric disjoint.
@@ -48,97 +48,97 @@ Module Local.
     econs. symmetry. apply H.
   Qed.
 
-  Inductive promise_step (th1:t) (mem1:Memory.t) (loc:Loc.t) (from to:Time.t) (val:Const.t) (released:Snapshot.t): forall (th2:t) (mem2:Memory.t), Prop :=
+  Inductive promise_step (lc1:t) (mem1:Memory.t) (loc:Loc.t) (from to:Time.t) (val:Const.t) (released:Snapshot.t): forall (lc2:t) (mem2:Memory.t), Prop :=
   | step_promise
       commit2 promise2 mem2
-      (COMMIT: Commit.le th1.(commit) commit2)
+      (COMMIT: Commit.le lc1.(commit) commit2)
       (COMMIT_WF: Commit.wf commit2 mem2)
-      (MEMORY: Memory.promise th1.(promise) mem1 loc from to (Message.mk val released) promise2 mem2):
-      promise_step th1 mem1 loc from to val released (mk commit2 promise2) mem2
+      (MEMORY: Memory.promise lc1.(promise) mem1 loc from to (Message.mk val released) promise2 mem2):
+      promise_step lc1 mem1 loc from to val released (mk commit2 promise2) mem2
   .
 
-  Inductive silent_step (th1:t) (mem1:Memory.t): forall (th2:t), Prop :=
+  Inductive silent_step (lc1:t) (mem1:Memory.t): forall (lc2:t), Prop :=
   | step_silent
       commit2
-      (COMMIT: Commit.le th1.(commit) commit2)
+      (COMMIT: Commit.le lc1.(commit) commit2)
       (COMMIT_WF: Commit.wf commit2 mem1):
-      silent_step th1 mem1 (mk commit2 th1.(promise))
+      silent_step lc1 mem1 (mk commit2 lc1.(promise))
   .
 
-  Inductive read_step (th1:t) (mem1:Memory.t) (loc:Loc.t) (ts:Time.t) (val:Const.t) (released:Snapshot.t) (ord:Ordering.t): forall (th2:t), Prop :=
+  Inductive read_step (lc1:t) (mem1:Memory.t) (loc:Loc.t) (ts:Time.t) (val:Const.t) (released:Snapshot.t) (ord:Ordering.t): forall (lc2:t), Prop :=
   | step_read
       commit2
-      (COMMIT: Commit.read th1.(commit) loc ts released ord commit2)
+      (COMMIT: Commit.read lc1.(commit) loc ts released ord commit2)
       (COMMIT_WF: Commit.wf commit2 mem1)
       (GET: Memory.get loc ts mem1 = Some (Message.mk val released))
-      (GET_PROMISE: Memory.get loc ts th1.(promise) = None):
-      read_step th1 mem1 loc ts val released ord (mk commit2 th1.(promise))
+      (GET_PROMISE: Memory.get loc ts lc1.(promise) = None):
+      read_step lc1 mem1 loc ts val released ord (mk commit2 lc1.(promise))
   .
 
-  Inductive fulfill_step (th1:t) (mem1:Memory.t) (loc:Loc.t) (from to:Time.t) (val:Const.t) (released:Snapshot.t) (ord:Ordering.t): forall (th2:t), Prop :=
+  Inductive fulfill_step (lc1:t) (mem1:Memory.t) (loc:Loc.t) (from to:Time.t) (val:Const.t) (released:Snapshot.t) (ord:Ordering.t): forall (lc2:t), Prop :=
   | step_fulfill
       commit2 promise2
-      (COMMIT: Commit.write th1.(commit) loc to released ord commit2)
+      (COMMIT: Commit.write lc1.(commit) loc to released ord commit2)
       (COMMIT_WF: Commit.wf commit2 mem1)
-      (MEMORY: Memory.fulfill th1.(promise) loc from to (Message.mk val released) promise2):
-      fulfill_step th1 mem1 loc from to val released ord (mk commit2 promise2)
+      (MEMORY: Memory.fulfill lc1.(promise) loc from to (Message.mk val released) promise2):
+      fulfill_step lc1 mem1 loc from to val released ord (mk commit2 promise2)
   .
 
-  Inductive write_step (th1:t) (mem1:Memory.t) (loc:Loc.t) (from to:Time.t) (val:Const.t) (released:Snapshot.t) (ord:Ordering.t): forall (th2:t) (mem2:Memory.t), Prop :=
+  Inductive write_step (lc1:t) (mem1:Memory.t) (loc:Loc.t) (from to:Time.t) (val:Const.t) (released:Snapshot.t) (ord:Ordering.t): forall (lc2:t) (mem2:Memory.t), Prop :=
   | step_write_fulfill
-      th2
-      (FULFILL: fulfill_step th1 mem1 loc from to val released ord th2)
-      (RELEASE: Ordering.le Ordering.acqrel ord -> th1.(promise) loc = Cell.bot):
-      write_step th1 mem1 loc from to val released ord th2 mem1
+      lc2
+      (FULFILL: fulfill_step lc1 mem1 loc from to val released ord lc2)
+      (RELEASE: Ordering.le Ordering.acqrel ord -> lc1.(promise) loc = Cell.bot):
+      write_step lc1 mem1 loc from to val released ord lc2 mem1
   | step_write_add
-      th2 mem2 th3
-      (PROMISE: promise_step th1 mem1 loc from to val released th2 mem2)
-      (FULFILL: fulfill_step th2 mem2 loc from to val released ord th3)
-      (RELEASE: Ordering.le Ordering.acqrel ord -> th1.(promise) loc = Cell.bot):
-      write_step th1 mem1 loc from to val released ord th3 mem2
+      lc2 mem2 lc3
+      (PROMISE: promise_step lc1 mem1 loc from to val released lc2 mem2)
+      (FULFILL: fulfill_step lc2 mem2 loc from to val released ord lc3)
+      (RELEASE: Ordering.le Ordering.acqrel ord -> lc1.(promise) loc = Cell.bot):
+      write_step lc1 mem1 loc from to val released ord lc3 mem2
   .
 
-  Inductive fence_step (th1:t) (mem1:Memory.t) (ordr ordw:Ordering.t): forall (th2:t), Prop :=
+  Inductive fence_step (lc1:t) (mem1:Memory.t) (ordr ordw:Ordering.t): forall (lc2:t), Prop :=
   | step_fence
       commit2
-      (COMMIT: Commit.fence th1.(commit) ordr ordw commit2)
+      (COMMIT: Commit.fence lc1.(commit) ordr ordw commit2)
       (COMMIT_WF: Commit.wf commit2 mem1)
-      (RELEASE: Ordering.le Ordering.acqrel ordw -> th1.(promise) = Memory.bot):
-      fence_step th1 mem1 ordr ordw (mk commit2 th1.(promise))
+      (RELEASE: Ordering.le Ordering.acqrel ordw -> lc1.(promise) = Memory.bot):
+      fence_step lc1 mem1 ordr ordw (mk commit2 lc1.(promise))
   .
 
-  Lemma future_read_step th1 mem1 mem1' loc ts val released ord th2
+  Lemma future_read_step lc1 mem1 mem1' loc ts val released ord lc2
         (FUTURE: Memory.future mem1 mem1')
-        (STEP: read_step th1 mem1 loc ts val released ord th2):
-    read_step th1 mem1' loc ts val released ord th2.
+        (STEP: read_step lc1 mem1 loc ts val released ord lc2):
+    read_step lc1 mem1' loc ts val released ord lc2.
   Proof.
     inv STEP. econs; eauto.
     - eapply Commit.future_wf; eauto.
     - eapply Memory.future_get; eauto.
   Qed.
 
-  Lemma future_fulfill_step th1 mem1 mem1' loc from to val released ord th2
+  Lemma future_fulfill_step lc1 mem1 mem1' loc from to val released ord lc2
         (FUTURE: Memory.future mem1 mem1')
-        (STEP: fulfill_step th1 mem1 loc from to val released ord th2):
-    fulfill_step th1 mem1' loc from to val released ord th2.
+        (STEP: fulfill_step lc1 mem1 loc from to val released ord lc2):
+    fulfill_step lc1 mem1' loc from to val released ord lc2.
   Proof.
     inv STEP. econs; eauto.
     eapply Commit.future_wf; eauto.
   Qed.
 
-  Lemma future_fence_step th1 mem1 mem1' ordr ordw th2
+  Lemma future_fence_step lc1 mem1 mem1' ordr ordw lc2
         (FUTURE: Memory.future mem1 mem1')
-        (STEP: fence_step th1 mem1 ordr ordw th2):
-    fence_step th1 mem1' ordr ordw th2.
+        (STEP: fence_step lc1 mem1 ordr ordw lc2):
+    fence_step lc1 mem1' ordr ordw lc2.
   Proof.
     inv STEP. econs; eauto.
     eapply Commit.future_wf; eauto.
   Qed.
 
-  Lemma promise_step_future th1 mem1 loc from to val released th2 mem2
-        (STEP: promise_step th1 mem1 loc from to val released th2 mem2)
-        (WF1: wf th1 mem1):
-    <<WF2: wf th2 mem2>> /\
+  Lemma promise_step_future lc1 mem1 loc from to val released lc2 mem2
+        (STEP: promise_step lc1 mem1 loc from to val released lc2 mem2)
+        (WF1: wf lc1 mem1):
+    <<WF2: wf lc2 mem2>> /\
     <<FUTURE: Memory.future mem1 mem2>>.
   Proof.
     inv WF1. inv STEP.
@@ -146,36 +146,36 @@ Module Local.
     splits; ss.
   Qed.
 
-  Lemma silent_step_future th1 mem1 th2
-        (STEP: silent_step th1 mem1 th2)
-        (WF1: wf th1 mem1):
-    wf th2 mem1.
+  Lemma silent_step_future lc1 mem1 lc2
+        (STEP: silent_step lc1 mem1 lc2)
+        (WF1: wf lc1 mem1):
+    wf lc2 mem1.
   Proof.
     inv WF1. inv STEP. ss.
   Qed.
 
-  Lemma read_step_future th1 mem1 loc ts val released ord th2
-        (STEP: read_step th1 mem1 loc ts val released ord th2)
-        (WF1: wf th1 mem1):
-    wf th2 mem1.
+  Lemma read_step_future lc1 mem1 loc ts val released ord lc2
+        (STEP: read_step lc1 mem1 loc ts val released ord lc2)
+        (WF1: wf lc1 mem1):
+    wf lc2 mem1.
   Proof.
     inv WF1. inv STEP. ss.
   Qed.
 
-  Lemma fulfill_step_future th1 mem1 loc from to val released ord th2
-        (STEP: fulfill_step th1 mem1 loc from to val released ord th2)
-        (WF1: wf th1 mem1):
-    wf th2 mem1.
+  Lemma fulfill_step_future lc1 mem1 loc from to val released ord lc2
+        (STEP: fulfill_step lc1 mem1 loc from to val released ord lc2)
+        (WF1: wf lc1 mem1):
+    wf lc2 mem1.
   Proof.
     inv WF1. inv STEP.
     exploit Memory.fulfill_future; eauto. i.
     splits; ss.
   Qed.
 
-  Lemma write_step_future th1 mem1 loc from to val released ord th2 mem2
-        (STEP: write_step th1 mem1 loc from to val released ord th2 mem2)
-        (WF1: wf th1 mem1):
-    <<WF2: wf th2 mem2>> /\
+  Lemma write_step_future lc1 mem1 loc from to val released ord lc2 mem2
+        (STEP: write_step lc1 mem1 loc from to val released ord lc2 mem2)
+        (WF1: wf lc1 mem1):
+    <<WF2: wf lc2 mem2>> /\
     <<FUTURE: Memory.future mem1 mem2>>.
   Proof.
     inv STEP.
@@ -184,22 +184,22 @@ Module Local.
       exploit fulfill_step_future; eauto.
   Qed.
 
-  Lemma fence_step_future th1 mem1 ordr ordw th2
-        (STEP: fence_step th1 mem1 ordr ordw th2)
-        (WF1: wf th1 mem1):
-    wf th2 mem1.
+  Lemma fence_step_future lc1 mem1 ordr ordw lc2
+        (STEP: fence_step lc1 mem1 ordr ordw lc2)
+        (WF1: wf lc1 mem1):
+    wf lc2 mem1.
   Proof.
     inv WF1. inv STEP. ss.
   Qed.
 
   Lemma promise_step_disjoint
-        th1 mem1 loc from to val released th2 mem2 th
-        (STEP: promise_step th1 mem1 loc from to val released th2 mem2)
-        (WF1: wf th1 mem1)
-        (DISJOINT1: disjoint th1 th)
-        (WF: wf th mem1):
-    <<DISJOINT2: disjoint th2 th>> /\
-    <<WF: wf th mem2>>.
+        lc1 mem1 loc from to val released lc2 mem2 lc
+        (STEP: promise_step lc1 mem1 loc from to val released lc2 mem2)
+        (WF1: wf lc1 mem1)
+        (DISJOINT1: disjoint lc1 lc)
+        (WF: wf lc mem1):
+    <<DISJOINT2: disjoint lc2 lc>> /\
+    <<WF: wf lc mem2>>.
   Proof.
     inv WF1. inv DISJOINT1. inv WF. inv STEP.
     exploit Memory.promise_future; try apply MEMORY1; eauto. i. des.
@@ -209,32 +209,32 @@ Module Local.
   Qed.
 
   Lemma silent_step_disjoint
-        th1 mem1 th2 th
-        (STEP: silent_step th1 mem1 th2)
-        (WF1: wf th1 mem1)
-        (DISJOINT1: disjoint th1 th)
-        (WF: wf th mem1):
-    disjoint th2 th.
+        lc1 mem1 lc2 lc
+        (STEP: silent_step lc1 mem1 lc2)
+        (WF1: wf lc1 mem1)
+        (DISJOINT1: disjoint lc1 lc)
+        (WF: wf lc mem1):
+    disjoint lc2 lc.
   Proof.
     inv WF1. inv DISJOINT1. inv WF. inv STEP. ss.
   Qed.
 
   Lemma read_step_disjoint
-        th1 mem1 th2 loc ts val released ord th
-        (STEP: read_step th1 mem1 loc ts val released ord th2)
-        (WF1: wf th1 mem1)
-        (DISJOINT1: disjoint th1 th)
-        (WF: wf th mem1):
-    disjoint th2 th.
+        lc1 mem1 lc2 loc ts val released ord lc
+        (STEP: read_step lc1 mem1 loc ts val released ord lc2)
+        (WF1: wf lc1 mem1)
+        (DISJOINT1: disjoint lc1 lc)
+        (WF: wf lc mem1):
+    disjoint lc2 lc.
   Proof.
     inv WF1. inv DISJOINT1. inv WF. inv STEP. ss.
   Qed.
 
   Lemma fulfill_step_disjoint
-        th1 mem1 th2 loc from to val released ord th
-        (STEP: fulfill_step th1 mem1 loc from to val released ord th2)
-        (DISJOINT1: disjoint th1 th):
-    disjoint th2 th.
+        lc1 mem1 lc2 loc from to val released ord lc
+        (STEP: fulfill_step lc1 mem1 loc from to val released ord lc2)
+        (DISJOINT1: disjoint lc1 lc):
+    disjoint lc2 lc.
   Proof.
     inv DISJOINT1. inv STEP. inv MEMORY.
     rewrite PROMISE1 in *. memtac.
@@ -242,13 +242,13 @@ Module Local.
   Qed.
 
   Lemma write_step_disjoint
-        th1 mem1 th2 loc from to val released ord mem2 th
-        (STEP: write_step th1 mem1 loc from to val released ord th2 mem2)
-        (WF1: wf th1 mem1)
-        (DISJOINT1: disjoint th1 th)
-        (WF: wf th mem1):
-    <<DISJOINT2: disjoint th2 th>> /\
-    <<WF: wf th mem2>>.
+        lc1 mem1 lc2 loc from to val released ord mem2 lc
+        (STEP: write_step lc1 mem1 loc from to val released ord lc2 mem2)
+        (WF1: wf lc1 mem1)
+        (DISJOINT1: disjoint lc1 lc)
+        (WF: wf lc mem1):
+    <<DISJOINT2: disjoint lc2 lc>> /\
+    <<WF: wf lc mem2>>.
   Proof.
     inv STEP.
     - splits; auto. eapply fulfill_step_disjoint; eauto.
@@ -258,12 +258,12 @@ Module Local.
   Qed.
 
   Lemma fence_step_disjoint
-        th1 mem1 th2 ordr ordw th
-        (STEP: fence_step th1 mem1 ordr ordw th2)
-        (WF1: wf th1 mem1)
-        (DISJOINT1: disjoint th1 th)
-        (WF: wf th mem1):
-    disjoint th2 th.
+        lc1 mem1 lc2 ordr ordw lc
+        (STEP: fence_step lc1 mem1 ordr ordw lc2)
+        (WF1: wf lc1 mem1)
+        (DISJOINT1: disjoint lc1 lc)
+        (WF: wf lc mem1):
+    disjoint lc2 lc.
   Proof.
     inv WF1. inv DISJOINT1. inv WF. inv STEP. ss.
   Qed.
@@ -281,49 +281,49 @@ Module Thread.
 
     Inductive promise_step (e1:t): forall (e2:t), Prop :=
     | promise_step_intro
-        loc from to val released th2 mem2
-        (LOCAL: Local.promise_step e1.(thread) e1.(memory) loc from to val released th2 mem2):
-        promise_step e1 (mk e1.(state) th2 mem2)
+        loc from to val released lc2 mem2
+        (LOCAL: Local.promise_step e1.(thread) e1.(memory) loc from to val released lc2 mem2):
+        promise_step e1 (mk e1.(state) lc2 mem2)
     .
 
     Inductive internal_step (e1:t): forall (e2:t), Prop :=
     | step_silent
-        st2 th2
+        st2 lc2
         (STATE: lang.(Language.step) None e1.(state) st2)
-        (LOCAL: Local.silent_step e1.(thread) e1.(memory) th2):
-        internal_step e1 (mk st2 th2 e1.(memory))
+        (LOCAL: Local.silent_step e1.(thread) e1.(memory) lc2):
+        internal_step e1 (mk st2 lc2 e1.(memory))
     | step_read
-        st2 loc ts val released ord th2
+        st2 loc ts val released ord lc2
         (STATE: lang.(Language.step) (Some (ThreadEvent.mem (MemEvent.read loc val ord))) e1.(state) st2)
-        (LOCAL: Local.read_step e1.(thread) e1.(memory) loc ts val released ord th2):
-        internal_step e1 (mk st2 th2 e1.(memory))
+        (LOCAL: Local.read_step e1.(thread) e1.(memory) loc ts val released ord lc2):
+        internal_step e1 (mk st2 lc2 e1.(memory))
     | step_write
-        st2 loc from to val released ord th2 mem2
+        st2 loc from to val released ord lc2 mem2
         (STATE: lang.(Language.step) (Some (ThreadEvent.mem (MemEvent.write loc val ord))) e1.(state) st2)
-        (LOCAL: Local.write_step e1.(thread) e1.(memory) loc from to val released ord th2 mem2):
-        internal_step e1 (mk st2 th2 mem2)
+        (LOCAL: Local.write_step e1.(thread) e1.(memory) loc from to val released ord lc2 mem2):
+        internal_step e1 (mk st2 lc2 mem2)
     | step_update
         st3 loc ordr ordw
-        tsr valr releasedr th2
-        tsw valw releasedw th3 mem3
+        tsr valr releasedr lc2
+        tsw valw releasedw lc3 mem3
         (STATE: lang.(Language.step) (Some (ThreadEvent.mem (MemEvent.update loc valr valw ordr ordw))) e1.(state) st3)
-        (LOCAL1: Local.read_step e1.(thread) e1.(memory) loc tsr valr releasedr ordr th2)
-        (LOCAL2: Local.write_step th2 e1.(memory) loc tsr tsw valw releasedw ordw th3 mem3)
+        (LOCAL1: Local.read_step e1.(thread) e1.(memory) loc tsr valr releasedr ordr lc2)
+        (LOCAL2: Local.write_step lc2 e1.(memory) loc tsr tsw valw releasedw ordw lc3 mem3)
         (RELEASE: Snapshot.le releasedr releasedw):
-        internal_step e1 (mk st3 th3 mem3)
+        internal_step e1 (mk st3 lc3 mem3)
     | step_fence
-        st2 ordr ordw th2
+        st2 ordr ordw lc2
         (STATE: lang.(Language.step) (Some (ThreadEvent.mem (MemEvent.fence ordr ordw))) e1.(state) st2)
-        (LOCAL: Local.fence_step e1.(thread) e1.(memory) ordr ordw th2):
-        internal_step e1 (mk st2 th2 e1.(memory))
+        (LOCAL: Local.fence_step e1.(thread) e1.(memory) ordr ordw lc2):
+        internal_step e1 (mk st2 lc2 e1.(memory))
     .
 
     Inductive external_step (e:Event.t) (e1:t): forall (e2:t), Prop :=
     | step_syscall
-        st2 th2
+        st2 lc2
         (STATE: lang.(Language.step) (Some (ThreadEvent.syscall e)) e1.(state) st2)
-        (LOCAL: Local.silent_step e1.(thread) e1.(memory) th2):
-        external_step e e1 (mk st2 th2 e1.(memory))
+        (LOCAL: Local.silent_step e1.(thread) e1.(memory) lc2):
+        external_step e e1 (mk st2 lc2 e1.(memory))
     .
 
     Inductive step: forall (e:option Event.t) (e1:t) (e2:t), Prop :=
@@ -341,12 +341,12 @@ Module Thread.
         step (Some e) e1 e2
     .
 
-    Definition consistent st1 th1 mem: Prop :=
+    Definition consistent st1 lc1 mem: Prop :=
       forall mem1
         (FUTURE: Memory.future mem mem1)
-        (WF: Local.wf th1 mem1),
+        (WF: Local.wf lc1 mem1),
       exists e2,
-        <<STEPS: rtc (step None) (mk st1 th1 mem1) e2>> /\
+        <<STEPS: rtc (step None) (mk st1 lc1 mem1) e2>> /\
         <<PROMISE: e2.(thread).(Local.promise) = Memory.bot>>.
 
     Lemma promise_step_future e1 e2
@@ -409,26 +409,26 @@ Module Thread.
         splits; ss. etrans; eauto.
     Qed.
 
-    Lemma promise_step_disjoint e1 e2 th
+    Lemma promise_step_disjoint e1 e2 lc
         (STEP: promise_step e1 e2)
         (WF1: Local.wf e1.(thread) e1.(memory))
-        (DISJOINT1: Local.disjoint e1.(thread) th)
-        (WF: Local.wf th e1.(memory)):
-      <<DISJOINT2: Local.disjoint e2.(thread) th>> /\
-      <<WF: Local.wf th e2.(memory)>>.
+        (DISJOINT1: Local.disjoint e1.(thread) lc)
+        (WF: Local.wf lc e1.(memory)):
+      <<DISJOINT2: Local.disjoint e2.(thread) lc>> /\
+      <<WF: Local.wf lc e2.(memory)>>.
     Proof.
       inv STEP.
       exploit Local.promise_step_future; eauto. i. des.
       eapply Local.promise_step_disjoint; eauto.
     Qed.
 
-    Lemma internal_step_disjoint e1 e2 th
+    Lemma internal_step_disjoint e1 e2 lc
         (STEP: internal_step e1 e2)
         (WF1: Local.wf e1.(thread) e1.(memory))
-        (DISJOINT1: Local.disjoint e1.(thread) th)
-        (WF: Local.wf th e1.(memory)):
-      <<DISJOINT2: Local.disjoint e2.(thread) th>> /\
-      <<WF: Local.wf th e2.(memory)>>.
+        (DISJOINT1: Local.disjoint e1.(thread) lc)
+        (WF: Local.wf lc e1.(memory)):
+      <<DISJOINT2: Local.disjoint e2.(thread) lc>> /\
+      <<WF: Local.wf lc e2.(memory)>>.
     Proof.
       inv STEP.
       - exploit Local.silent_step_future; eauto. i.
@@ -445,25 +445,25 @@ Module Thread.
         exploit Local.fence_step_disjoint; eauto.
     Qed.
 
-    Lemma external_step_disjoint e e1 e2 th
+    Lemma external_step_disjoint e e1 e2 lc
         (STEP: external_step e e1 e2)
         (WF1: Local.wf e1.(thread) e1.(memory))
-        (DISJOINT1: Local.disjoint e1.(thread) th)
-        (WF: Local.wf th e1.(memory)):
-      <<DISJOINT2: Local.disjoint e2.(thread) th>> /\
-      <<WF: Local.wf th e2.(memory)>>.
+        (DISJOINT1: Local.disjoint e1.(thread) lc)
+        (WF: Local.wf lc e1.(memory)):
+      <<DISJOINT2: Local.disjoint e2.(thread) lc>> /\
+      <<WF: Local.wf lc e2.(memory)>>.
     Proof.
       inv STEP. exploit Local.silent_step_future; eauto. i.
       exploit Local.silent_step_disjoint; eauto.
     Qed.
 
-    Lemma step_disjoint e e1 e2 th
+    Lemma step_disjoint e e1 e2 lc
         (STEP: step e e1 e2)
         (WF1: Local.wf e1.(thread) e1.(memory))
-        (DISJOINT1: Local.disjoint e1.(thread) th)
-        (WF: Local.wf th e1.(memory)):
-      <<DISJOINT2: Local.disjoint e2.(thread) th>> /\
-      <<WF: Local.wf th e2.(memory)>>.
+        (DISJOINT1: Local.disjoint e1.(thread) lc)
+        (WF: Local.wf lc e1.(memory)):
+      <<DISJOINT2: Local.disjoint e2.(thread) lc>> /\
+      <<WF: Local.wf lc e2.(memory)>>.
     Proof.
       inv STEP.
       - eapply promise_step_disjoint; eauto.
@@ -471,13 +471,13 @@ Module Thread.
       - eapply external_step_disjoint; eauto.
     Qed.
 
-    Lemma rtc_step_disjoint e1 e2 th
+    Lemma rtc_step_disjoint e1 e2 lc
         (STEP: rtc (step None) e1 e2)
         (WF1: Local.wf e1.(thread) e1.(memory))
-        (DISJOINT1: Local.disjoint e1.(thread) th)
-        (WF: Local.wf th e1.(memory)):
-      <<DISJOINT2: Local.disjoint e2.(thread) th>> /\
-      <<WF: Local.wf th e2.(memory)>>.
+        (DISJOINT1: Local.disjoint e1.(thread) lc)
+        (WF: Local.wf lc e1.(memory)):
+      <<DISJOINT2: Local.disjoint e2.(thread) lc>> /\
+      <<WF: Local.wf lc e2.(memory)>>.
     Proof.
       revert WF1 DISJOINT1 WF. induction STEP; eauto. i.
       exploit step_future; eauto. i. des.
