src/opt/ReorderStore.v
@@ -50,34 +50,34 @@ Inductive reorder_store l1 v1 o1: forall (i2:Instr.t), Prop :=
     reorder_store l1 v1 o1 (Instr.update r2 l2 rmw2 or2 ow2)
 .
 
-Inductive sim_store: forall (st_src:lang.(Language.state)) (th_src:Local.t) (mem_k_src:Memory.t)
-                       (st_tgt:lang.(Language.state)) (th_tgt:Local.t) (mem_k_tgt:Memory.t), Prop :=
+Inductive sim_store: forall (st_src:lang.(Language.state)) (lc_src:Local.t) (mem_k_src:Memory.t)
+                       (st_tgt:lang.(Language.state)) (lc_tgt:Local.t) (mem_k_tgt:Memory.t), Prop :=
 | sim_store_intro
     l1 f1 t1 v1 released1 o1 i2
-    rs th1_src th1_tgt th2_src
+    rs lc1_src lc1_tgt lc2_src
     mem_k_src mem_k_tgt
     (REORDER: reorder_store l1 v1 o1 i2)
-    (FULFILL: Local.fulfill_step th1_src mem_k_src l1 f1 t1 (RegFile.eval_value rs v1) released1 o1 th2_src)
-    (LOCAL: sim_local th2_src th1_tgt):
+    (FULFILL: Local.fulfill_step lc1_src mem_k_src l1 f1 t1 (RegFile.eval_value rs v1) released1 o1 lc2_src)
+    (LOCAL: sim_local lc2_src lc1_tgt):
     sim_store
-      (State.mk rs [Stmt.instr i2; Stmt.instr (Instr.store l1 v1 o1)]) th1_src mem_k_src
-      (State.mk rs [Stmt.instr i2]) th1_tgt mem_k_tgt
+      (State.mk rs [Stmt.instr i2; Stmt.instr (Instr.store l1 v1 o1)]) lc1_src mem_k_src
+      (State.mk rs [Stmt.instr i2]) lc1_tgt mem_k_tgt
 .
 
 Lemma sim_store_step
-      st1_src th1_src mem_k_src
-      st1_tgt th1_tgt mem_k_tgt
-      (SIM: sim_store st1_src th1_src mem_k_src
-                      st1_tgt th1_tgt mem_k_tgt):
+      st1_src lc1_src mem_k_src
+      st1_tgt lc1_tgt mem_k_tgt
+      (SIM: sim_store st1_src lc1_src mem_k_src
+                      st1_tgt lc1_tgt mem_k_tgt):
   forall mem1_src mem1_tgt
     (MEMORY: sim_memory mem1_src mem1_tgt)
     (FUTURE_SRC: Memory.future mem_k_src mem1_src)
     (FUTURE_TGT: Memory.future mem_k_tgt mem1_tgt)
-    (WF_SRC: Local.wf th1_src mem1_src)
-    (WF_TGT: Local.wf th1_tgt mem1_tgt),
+    (WF_SRC: Local.wf lc1_src mem1_src)
+    (WF_TGT: Local.wf lc1_tgt mem1_tgt),
     _sim_thread_step lang lang ((sim_thread (sim_terminal eq)) \6/ sim_store)
-                     st1_src th1_src mem1_src
-                     st1_tgt th1_tgt mem1_tgt.
+                     st1_src lc1_src mem1_src
+                     st1_tgt lc1_tgt mem1_tgt.
 Proof.
   inv SIM. ii.
   exploit Local.future_fulfill_step; try apply FULFILL; eauto. i.
@@ -159,7 +159,7 @@ Proof.
   - inversion PR. subst. i.
     exploit (progress_step rs i2 nil); eauto.
     i. des; [|by inv STEP; inv STATE; inv INSTR; inv REORDER].
-    destruct th2. exploit sim_store_step; eauto.
+    destruct lc2. exploit sim_store_step; eauto.
     { econs 2. eauto. }
     i. des.
     + exploit internal_step_promise; eauto. i.
